feat: prove array_existence under heap modification

isabelle/Hoare/InsertionSort.thy
@@ -2,9 +2,89 @@ theory InsertionSort
   imports Main "HOL-Hoare.Separation"
 begin
 
+fun swapAt where
+  "swapAt i j xs = list_update (list_update xs i (xs ! j)) j (xs ! i)"
+
+lemma swapAt_same: "i < length xs \<Longrightarrow> swapAt i i xs = xs"
+  apply (induct xs)
+  apply simp
+  apply simp
+  done
+
 inductive array where
   "array H p 0 []"
 | "H p = Some a \<Longrightarrow> array H (p+1) k as \<Longrightarrow> array H p (Suc k) (a#as)"
+
+lemma array_length:
+  "array H p k xs \<Longrightarrow> length xs = k"
+  apply (induct rule: array.induct)
+  apply auto
+  done
+
+lemma array_singleton:
+  assumes "array H p 1 xs"
+  obtains x where "xs = [x]"
+  using assms
+  by (metis One_nat_def array.cases nat.simps(1) nat.simps(3))
+
+lemma array_empty_from: "array H p n [] \<Longrightarrow> n = 0"
+  apply (cases n)
+  apply simp
+  apply simp
+  using array_length by force
+
+lemma array_exists_under_heap_modification:
+  assumes "array H p n xs"
+  obtains zs where "array (H(x \<mapsto> y)) p n zs" "\<And>i. i < n \<Longrightarrow> if x = p + i then zs ! i = y else zs ! i = xs ! i"
+proof-
+  have "array H p n xs \<Longrightarrow> \<exists>zs. array (H(x \<mapsto> y)) p n zs \<and> (\<forall>i. i < n \<longrightarrow> (if x = p + i then zs ! i = y else zs ! i = xs ! i))"
+    apply (induct rule: array.induct)
+    using array.intros(1) apply blast
+  proof-
+    fix H p a k as
+    assume "H p = Some a" "array H (p + 1) k as"
+    and "\<exists>zs. array (H(x \<mapsto> y)) (p + 1) k zs \<and> (\<forall>i<k. if x = p + 1 + i then zs ! i = y else zs ! i = as ! i)"
+    obtain zs where "array (H(x \<mapsto> y)) (p + 1) k zs \<and> (\<forall>i<k. if x = p + 1 + i then zs ! i = y else zs ! i = as ! i)"
+      using \<open>\<exists>zs. array (H(x \<mapsto> y)) (p + 1) k zs \<and> (\<forall>i<k. if x = p + 1 + i then zs ! i = y else zs ! i = as ! i)\<close> by blast
+    have "length zs = k"
+      using \<open>array (H(x \<mapsto> y)) (p + 1) k zs \<and> (\<forall>i<k. if x = p + 1 + i then zs ! i = y else zs ! i = as ! i)\<close> array_length by blast
+
+    { assume "p = x"
+      have "\<And>i. i < k \<Longrightarrow> x \<noteq> p + 1 + i"
+        by (simp add: \<open>p = x\<close>)
+      hence "\<And>i. i < k \<Longrightarrow> zs ! i = as ! i"
+        by (simp add: \<open>array (H(x \<mapsto> y)) (p + 1) k zs \<and> (\<forall>i<k. if x = p + 1 + i then zs ! i = y else zs ! i = as ! i)\<close>)
+      hence "zs = as"
+        by (metis \<open>array H (p + 1) k as\<close> \<open>length zs = k\<close> array_length list_eq_iff_nth_eq)
+
+      have "array (H(x \<mapsto> y)) p (Suc k) (y # zs) \<and> (\<forall>i<Suc k. if x = p + i then (y # zs) ! i = y else (y # zs) ! i = (a # as) ! i)"
+        by (metis \<open>array (H(x \<mapsto> y)) (p + 1) k zs \<and> (\<forall>i<k. if x = p + 1 + i then zs ! i = y else zs ! i = as ! i)\<close> \<open>p = x\<close> \<open>zs = as\<close> add.right_neutral add_left_cancel array.intros(2) fun_upd_same nth_Cons')
+    }
+    hence "p = x \<Longrightarrow> array (H(x \<mapsto> y)) p (Suc k) (y # zs) \<and> (\<forall>i<Suc k. if x = p + i then (y # zs) ! i = y else (y # zs) ! i = (a # as) ! i)"
+      by blast
+
+    { assume "p \<noteq> x"
+
+      have "array (H(x \<mapsto> y)) p (Suc k) (a # zs) \<and> (\<forall>i<Suc k. if x = p + i then (a # zs) ! i = y else (a # zs) ! i = (a # as) ! i)"
+        by (smt \<open>H p = Some a\<close> \<open>array (H(x \<mapsto> y)) (p + 1) k zs \<and> (\<forall>i<k. if x = p + 1 + i then zs ! i = y else zs ! i = as ! i)\<close> \<open>p \<noteq> x\<close> add.right_neutral add_diff_cancel_left' array.intros(2) group_cancel.add1 less_Suc_eq_0_disj map_upd_Some_unfold nth_Cons_0 nth_Cons_pos plus_1_eq_Suc)
+    }
+    hence "p \<noteq> x \<Longrightarrow> array (H(x \<mapsto> y)) p (Suc k) (a # zs) \<and> (\<forall>i<Suc k. if x = p + i then (a # zs) ! i = y else (a # zs) ! i = (a # as) ! i)"
+      by blast
+
+    show "\<exists>zs. array (H(x \<mapsto> y)) p (Suc k) zs \<and> (\<forall>i<Suc k. if x = p + i then zs ! i = y else zs ! i = (a # as) ! i)"
+      using \<open>p = x \<Longrightarrow> array (H(x \<mapsto> y)) p (Suc k) (y # zs) \<and> (\<forall>i<Suc k. if x = p + i then (y # zs) ! i = y else (y # zs) ! i = (a # as) ! i)\<close> \<open>p \<noteq> x \<Longrightarrow> array (H(x \<mapsto> y)) p (Suc k) (a # zs) \<and> (\<forall>i<Suc k. if x = p + i then (a # zs) ! i = y else (a # zs) ! i = (a # as) ! i)\<close> by blast
+  qed
+
+  show "(\<And>zs. array (H(x \<mapsto> y)) p n zs \<Longrightarrow> (\<And>i. i < n \<Longrightarrow> if x = p + i then zs ! i = y else zs ! i = xs ! i) \<Longrightarrow> thesis) \<Longrightarrow> thesis"
+    using assms
+    using \<open>array H p n xs \<Longrightarrow> \<exists>zs. array (H(x \<mapsto> y)) p n zs \<and> (\<forall>i<n. if x = p + i then zs ! i = y else zs ! i = xs ! i)\<close> by blast
+qed
+
+lemma array_swap_at:
+  assumes "array H p n xs" "i < length xs" "j < length xs"
+  shows "array (H(p + i \<mapsto> the (H (p + j)), p + j \<mapsto> the (H (p + i)))) p n (swapAt i j xs)"
+proof-
+  obtain zs where "array (H(p + i \<mapsto> the (H (p + j)), p + j \<mapsto> the (H (p + i)))) p n zs"
 
 primrec count where
   "count a [] = 0"
@@ -13,13 +93,22 @@ primrec count where
 definition permute where
   "permute xs ys \<equiv> (\<forall>a. count a xs = count a ys)"
 
+primrec head_swap_with where
+  "head_swap_with [] y = [y]"
+| "head_swap_with (x#xs) y = x#y#xs"
+
+fun removeAt where
+  "removeAt i xs = take (i-1) xs @ drop (i+1) xs"
+
 lemma "
-  VARS H i j
+  VARS H i j tmp
   {array H arr N xs}
   i := 1;
-  WHILE i < N INV {emp} DO
+  WHILE i < N
+  INV {\<exists>zs. array H arr (i - 1) zs \<and> sorted zs} DO
     j := i;
-    WHILE j > 0 & the (H (arr + j - 1)) > the (H (arr + j)) INV {emp} DO
+    WHILE j > 0 & the (H (arr + j - 1)) > the (H (arr + j))
+    INV {\<exists>zs'. j \<le> i \<and> array H arr (i - 1) zs' \<and> sorted (removeAt j zs')} DO
       tmp := the (H (arr + j));
       H := H (arr + j \<mapsto> the (H (arr + j - 1)));
       H := H (arr + j - 1 \<mapsto> tmp);
@@ -29,6 +118,123 @@ lemma "
   OD
   {array H arr N ys \<and> sorted ys \<and> permute xs ys}
 "
-  sorry
+  apply vcg
+proof-
+  show "\<And>H i j tmp. array H arr N xs \<Longrightarrow> \<exists>zs. array H arr (1 - 1) zs \<and> sorted zs"
+    apply simp
+    using array.intros(1) sorted.simps(1) by blast
+  show "\<And>H i j tmp. (\<exists>zs. array H arr (i - 1) zs \<and> sorted zs) \<and> i < N \<Longrightarrow> \<exists>zs'. i \<le> i \<and> array H arr (i - 1) zs' \<and> sorted (removeAt i zs')"
+    sorry
+
+  show "\<And>H i j tmp.
+       (\<exists>zs'. j \<le> i \<and> array H arr (i - 1) zs' \<and> sorted (removeAt j zs')) \<and> 0 < j \<and> the (H (arr + j)) < the (H (arr + j - 1)) \<Longrightarrow>
+       \<exists>zs'. j - 1 \<le> i \<and> array (H(arr + j \<mapsto> the (H (arr + j - 1)), arr + j - 1 \<mapsto> the (H (arr + j)))) arr (i - 1) zs' \<and> sorted (removeAt (j - 1) zs')"
+  proof-
+    fix H i j tmp
+    assume "(\<exists>zs'. j \<le> i \<and> array H arr (i - 1) zs' \<and> sorted (removeAt j zs')) \<and> 0 < j \<and> the (H (arr + j)) < the (H (arr + j - 1))"
+    obtain zs' where "j \<le> i \<and> array H arr (i - 1) zs' \<and> sorted (removeAt j zs')"
+      using \<open>(\<exists>zs'. j \<le> i \<and> array H arr (i - 1) zs' \<and> sorted (removeAt j zs')) \<and> 0 < j \<and> the (H (arr + j)) < the (H (arr + j - 1))\<close> by blast
+    have "j - 1 \<le> i"
+      using \<open>j \<le> i \<and> array H arr (i - 1) zs' \<and> sorted (removeAt j zs')\<close> le_diff_conv trans_le_add1 by blast
+    define zs where "zs \<equiv> swapAt j (j - 1) zs'"
+    have "array (H(arr + j \<mapsto> the (H (arr + j - 1)), arr + j - 1 \<mapsto> the (H (arr + j)))) arr (i - 1) zs"
+      apply (simp add: zs_def)
+
+    show "\<exists>zs'. j - 1 \<le> i \<and> array (H(arr + j \<mapsto> the (H (arr + j - 1)), arr + j - 1 \<mapsto> the (H (arr + j)))) arr (i - 1) zs' \<and> sorted (removeAt (j - 1) zs')"
+
+  show "\<And>H i j tmp.
+       (\<exists>k zs1 zs2.
+           k < j \<and>
+           j \<le> i \<and>
+           array H arr k zs1 \<and>
+           the (H (arr + k)) \<le> Min (set zs1) \<and> array H (arr + k) (i - k) zs2 \<and> Min (set (removeAt (j - k) zs2)) \<le> the (H (arr + k))) \<and>
+       0 < j \<and> the (H (arr + j)) < the (H (arr + j - 1)) \<Longrightarrow>
+       \<exists>k zs1 zs2.
+          k < j - 1 \<and>
+          j - 1 \<le> i \<and>
+          array (H(arr + j \<mapsto> the (H (arr + j - 1)), arr + j - 1 \<mapsto> the (H (arr + j)))) arr k zs1 \<and>
+          the ((H(arr + j \<mapsto> the (H (arr + j - 1)), arr + j - 1 \<mapsto> the (H (arr + j)))) (arr + k)) \<le> Min (set zs1) \<and>
+          array (H(arr + j \<mapsto> the (H (arr + j - 1)), arr + j - 1 \<mapsto> the (H (arr + j)))) (arr + k) (i - k) zs2 \<and>
+          Min (set (removeAt (j - 1 - k) zs2)) \<le> the ((H(arr + j \<mapsto> the (H (arr + j - 1)), arr + j - 1 \<mapsto> the (H (arr + j)))) (arr + k))"
+  proof-
+    fix H i j tmp
+    assume "(\<exists>k zs1 zs2.
+           k < j \<and>
+           j \<le> i \<and>
+           array H arr k zs1 \<and>
+           the (H (arr + k)) \<le> Min (set zs1) \<and> array H (arr + k) (i - k) zs2 \<and> Min (set (removeAt (j - k) zs2)) \<le> the (H (arr + k))) \<and>
+       0 < j \<and> the (H (arr + j)) < the (H (arr + j - 1))"
+    obtain k zs1 zs2 where "k < j \<and>
+           j \<le> i \<and>
+           array H arr k zs1 \<and>
+           the (H (arr + k)) \<le> Min (set zs1) \<and> array H (arr + k) (i - k) zs2 \<and> Min (set (removeAt (j - k) zs2)) \<le> the (H (arr + k))"
+      using \<open>(\<exists>k zs1 zs2. k < j \<and> j \<le> i \<and> array H arr k zs1 \<and> the (H (arr + k)) \<le> Min (set zs1) \<and> array H (arr + k) (i - k) zs2 \<and> Min (set (removeAt (j - k) zs2)) \<le> the (H (arr + k))) \<and> 0 < j \<and> the (H (arr + j)) < the (H (arr + j - 1))\<close> by blast
+    have "k = j - 1 \<Longrightarrow> False"
+    proof-
+      assume "k = j - 1"
+      have ""
+
+    show "\<exists>k zs1 zs2.
+          k < j - 1 \<and>
+          j - 1 \<le> i \<and>
+          array (H(arr + j \<mapsto> the (H (arr + j - 1)), arr + j - 1 \<mapsto> the (H (arr + j)))) arr k zs1 \<and>
+          the ((H(arr + j \<mapsto> the (H (arr + j - 1)), arr + j - 1 \<mapsto> the (H (arr + j)))) (arr + k)) \<le> Min (set zs1) \<and>
+          array (H(arr + j \<mapsto> the (H (arr + j - 1)), arr + j - 1 \<mapsto> the (H (arr + j)))) (arr + k) (i - k) zs2 \<and>
+          Min (set (removeAt (j - 1 - k) zs2)) \<le> the ((H(arr + j \<mapsto> the (H (arr + j - 1)), arr + j - 1 \<mapsto> the (H (arr + j)))) (arr + k))"
+
+  show "\<And>H i j tmp.
+       (\<exists>zs'. 0 < j \<and> j \<le> i \<and> array H (arr + j) (i - j) zs' \<and> sorted zs') \<and> 0 < j \<and> the (H (arr + j)) < the (H (arr + j - 1)) \<Longrightarrow>
+       \<exists>zs'. 0 < j - 1 \<and>
+             j - 1 \<le> i \<and> array (H(arr + j \<mapsto> the (H (arr + j - 1)), arr + j - 1 \<mapsto> the (H (arr + j)))) (arr + (j - 1)) (i - (j - 1)) zs' \<and> sorted zs'"
+  proof-
+    fix H and i j tmp
+    assume "(\<exists>zs'. 0 < j \<and> j \<le> i \<and> array H (arr + j) (i - j) zs' \<and> sorted zs') \<and> 0 < j \<and> the (H (arr + j)) < the (H (arr + j - 1))"
+    obtain zs where "0 < j \<and> j \<le> i \<and> array H (arr + j) (i - j) zs \<and> sorted zs"
+      using \<open>(\<exists>zs'. 0 < j \<and> j \<le> i \<and> array H (arr + j) (i - j) zs' \<and> sorted zs') \<and> 0 < j \<and> the (H (arr + j)) < the (H (arr + j - 1))\<close> by blast
+    define zs' where "zs' \<equiv> head_swap_with zs (the (H (arr + j - 1)))"
+
+    have "array (H(arr + j \<mapsto> the (H (arr + j - 1)), arr + j - 1 \<mapsto> the (H (arr + j)))) (arr + j - 1) (i - (j - 1)) zs'"
+      apply (simp add: zs'_def)
+      apply (cases zs)
+    proof-
+      assume "zs = []"
+      have "i = j"
+        using \<open>0 < j \<and> j \<le> i \<and> array H (arr + j) (i - j) zs \<and> sorted zs\<close> \<open>zs = []\<close> array_empty_from diff_is_0_eq le_antisym by blast
+      hence h: "i - (j - Suc 0) = 1"
+        by (simp add: Suc_leI \<open>(\<exists>zs'. 0 < j \<and> j \<le> i \<and> array H (arr + j) (i - j) zs' \<and> sorted zs') \<and> 0 < j \<and> the (H (arr + j)) < the (H (arr + j - 1))\<close>)
+
+      have h2: "head_swap_with zs (the (H (arr + j - Suc 0))) = [the (H (arr + j - Suc 0))]"
+        by (simp add: \<open>zs = []\<close>)
+
+      show "array (H(arr + j \<mapsto> the (H (arr + j - Suc 0)), arr + j - Suc 0 \<mapsto> the (H (arr + j)))) (arr + j - Suc 0) (i - (j - Suc 0)) 
+        (head_swap_with zs (the (H (arr + j - Suc 0))))"
+        apply (simp add: h h2)
+        apply rule
+        apply (simp add: Suc_leI \<open>(\<exists>zs'. 0 < j \<and> j \<le> i \<and> array H (arr + j) (i - j) zs' \<and> sorted zs') \<and> 0 < j \<and> the (H (arr + j)) < the (H (arr + j - 1))\<close>)
+        apply rule
+        done
+    next
+      fix a as
+      assume "zs = a # as"
+      have h: "head_swap_with zs (the (H (arr + j - Suc 0))) = a # the (H (arr + j - Suc 0)) # as"
+        by (simp add: \<open>zs = a # as\<close>)
+      have a: "a = the (H (arr + j))"
+        by (metis \<open>0 < j \<and> j \<le> i \<and> array H (arr + j) (i - j) zs \<and> sorted zs\<close> \<open>zs = a # as\<close> array.cases list.discI nth_Cons_0 option.sel)
+
+      have "array H (arr + j + 1) (i - j - 1) as"
+        by (metis One_nat_def \<open>0 < j \<and> j \<le> i \<and> array H (arr + j) (i - j) zs \<and> sorted zs\<close> \<open>zs = a # as\<close> add_diff_cancel_right' add_is_0 array.cases array_length list.inject list.size(4) nat.simps(3))
+
+      have "i - j \<ge> 1"
+        using \<open>0 < j \<and> j \<le> i \<and> array H (arr + j) (i - j) zs \<and> sorted zs\<close> \<open>zs = a # as\<close> array_length by fastforce
+      obtain k where k: "i - (j - Suc 0) = Suc (Suc k)"
+        using Suc_diff_le \<open>(\<exists>zs'. 0 < j \<and> j \<le> i \<and> array H (arr + j) (i - j) zs' \<and> sorted zs') \<and> 0 < j \<and> the (H (arr + j)) < the (H (arr + j - 1))\<close> \<open>1 \<le> i - j\<close> diff_Suc_1 by fastforce
+
+      show "array (H(arr + j \<mapsto> the (H (arr + j - Suc 0)), arr + j - Suc 0 \<mapsto> the (H (arr + j)))) (arr + j) (i - (j - Suc 0))
+        (head_swap_with zs (the (H (arr + j - Suc 0))))"
+        apply (simp add: h k)
+        apply rule
+        apply (simp add: a)
+
+    show "\<exists>zs'. j - 1 \<le> i \<and> array (H(arr + j \<mapsto> the (H (arr + j - 1)), arr + j - 1 \<mapsto> the (H (arr + j)))) (arr + (j - 1)) (i - (j - 1)) zs' \<and> sorted zs'"
 
 end
